Tries hnf

proof/Hnf.v
@@ -1,3 +1,5 @@
+Require Import Lambda.Utils.
+Require Import Lambda.Tactics.
 Require Import Lambda.Terms.
 Require Import Lambda.LiftSubst.
 Require Import Lambda.Reduction.
@@ -10,6 +12,41 @@ Implicit Types i k m n : nat.
 Implicit Type s : sort.
 Implicit Types A B M N T t u v : term.
 
+(*Definition head_elim (x : term) :=
+  match x with
+  App _ _ => True
+  | Pi1 _ => True
+  | Pi2 _ => True
+  | _ => False
+  end.
+
+Inductive in_hnf : term -> Prop :=
+  | hnf_beta : forall f, in_hnf f ->
+    (forall T b, f <> Abs T b) -> forall e, in_hnf (App f e)
+  | hnf_pi1 :  forall p, in_hnf p ->
+    (forall T x y, p <> Pair T x y) -> 
+    in_hnf (Pi1 p)
+  | hnf_pi2 :  forall p, in_hnf p ->
+    (forall T x y, p <> Pair T x y) -> 
+    in_hnf (Pi2 p)
+  | hnf_other : forall x, ~ (head_elim x) -> in_hnf x.
+
+Lemma hnf : forall x, exists y, red x y /\ in_hnf y.
+Proof.
+  intros.
+
+  induction x.
+
+  exists (Srt s) ; split ; [auto with coc | eapply hnf_other ; red ; simpl ; intros ; auto].
+
+  exists (Ref n) ; split ; [auto with coc | eapply hnf_other ; red ; simpl ; intros ; auto].
+
+  exists (Abs x1 x2) ; split ; [auto with coc | eapply hnf_other ; red ; simpl ; intros ; auto].
+
+  destruct_exists.
+  destruct x0.
+
+
 Fixpoint redex (x : term) :=
   match x with
   App (Abs _ _) _ => True
@@ -20,10 +57,54 @@ Fixpoint redex (x : term) :=
   | Pi2 x => redex x
   | _ => False
   end.
+*)
 
-Axiom hnf_measure : term -> nat.
+Definition redn := transp _ red1.
 
-Program Fixpoint hnf (x : term) { measure x hnf_measure } : term :=
+Definition snterm := { x : term | sn x }.
+
+Program Definition redn_sn : snterm -> snterm -> Prop := 
+  fun x y => (transp _ red1) x y.
+
+Definition sn_term_sn : forall t : snterm, sn (proj1_sig t).
+Proof.
+  destruct t ; auto.
+Qed.
+
+Scheme acc_dep := Induction for Acc Sort Prop.
+
+Lemma well_founded_redn_sn : well_founded redn_sn.
+Proof.
+  red in |- *.
+  cut (forall t u : snterm, redn_sn t u -> Acc redn_sn u).
+  intros.
+  apply H with a.
+
+  unfold redn_sn.
+  intros.
+  induction a.
+  unfold sn in p.
+  
+  induction p using acc_dep.
+  pose (H x).
+
+  inversion p.
+
+  simpl ; intros.
+
+  apply Acc_intro.
+  intros.
+  induction y.
+  simpl.
+  simpl in H.
+  
+
+
+  apply Acc_intro.
+  intros.
+  simpl in H0.
+
+Program Fixpoint hnf (x : snterm) { wf x redn_sn } : term :=
   match x with
   | App x y => 
     match hnf x with
@@ -44,8 +125,26 @@ Program Fixpoint hnf (x : term) { measure x hnf_measure } : term :=
   end.
 
 Obligation 1.
-  simpl ; subst ; intros.
-  subst.
+  simpl ; intros.
+
+  unfold well_founded.
+  unfold snterm.
+  intros.
+  induction a.
+  unfold sn in p.
+  inversion p.
+
+  apply Acc_intro.
+  intros.
+  unfold redn_sn in H ; simpl in H.
+  inversion p.
+  pose (H0 _ H).
+  
+  destruct y.
+  
+  simpl in a.
+  inversion a.
+
 
 
 Inductive hnf : term -> term -> Prop :=
